Carrier/KozenExample.thy
@@ -1,0 +1,615 @@
+theory KozenExample
+  imports Ranked_Alphabet List
+begin
+
+(* Kozen and Angus's example *)
+
+(* Defining the alphabet *)
+
+definition biconditional ::
+  "'a::ranked_alphabet skat \<Rightarrow> 'a skat \<Rightarrow> 'a skat" (infixl "iff" 65)
+where
+  "x iff y = !((x + y) \<cdot> !(x \<cdot> y))"
+
+declare biconditional_def [skat_simp]
+
+definition concat_map where "concat_map f = concat \<circ> map f"
+
+declare concat_map_def [simp]
+
+fun linsert :: "nat \<Rightarrow> 'a \<Rightarrow> 'a list \<Rightarrow> 'a list" where
+  "linsert 0 x ys = x#ys"
+| "linsert (Suc n) x (y#ys) = y # linsert n x ys"
+
+fun permute_step :: "'a \<Rightarrow> 'a list \<Rightarrow> 'a list list" where
+  "permute_step x [] = [[x]]"
+| "permute_step x (y#ys) = (x#y#ys) # (map (op # y) (permute_step x ys))"
+
+fun permute :: "'a list \<Rightarrow> 'a list list" where
+  "permute [] = [[]]"
+| "permute (x#xs) = concat_map (permute_step x) (permute xs)"
+
+datatype kzp = f_kzp | g_kzp | P_kzp | bot_kzp | x_kzp
+
+lemma kzp_UNIV: "UNIV = {P_kzp,f_kzp,g_kzp,bot_kzp,x_kzp}"
+  by (auto, metis kzp.exhaust)
+
+instantiation kzp :: ranked_alphabet
+begin
+
+  fun arity_kzp :: "kzp \<Rightarrow> nat" where
+    "arity_kzp f_kzp = 1"
+  | "arity_kzp g_kzp = 2"
+  | "arity_kzp P_kzp = 1"
+  | "arity_kzp bot_kzp = 0"
+  | "arity_kzp x_kzp = 0"
+
+  definition funs_kzp :: "kzp set" where "funs_kzp \<equiv> {f_kzp, g_kzp, bot_kzp, x_kzp}"
+
+  definition rels_kzp :: "kzp set" where "rels_kzp \<equiv> {P_kzp}"
+
+  definition NULL_kzp :: "kzp" where "NULL_kzp \<equiv> bot_kzp"
+
+  declare funs_kzp_def [skat_alphabet]
+    and rels_kzp_def [skat_alphabet]
+    and NULL_kzp_def [skat_alphabet]
+
+  definition output_vars_kzp :: "kzp itself \<Rightarrow> nat set" where "output_vars_kzp x \<equiv> {0}"
+
+  instance proof
+    show "finite (UNIV::kzp set)" by (simp add: kzp_UNIV)
+
+    show "(funs :: kzp set) \<inter> rels = {}"
+      by (simp add: funs_kzp_def rels_kzp_def)
+
+    show "(funs :: kzp set) \<union> rels = UNIV"
+      by (simp add: funs_kzp_def rels_kzp_def kzp_UNIV)
+
+    show "(funs :: kzp set) \<noteq> {}"
+      by (simp add: funs_kzp_def)
+
+    show "(rels :: kzp set) \<noteq> {}"
+      by (simp add: rels_kzp_def)
+
+    show "NULL \<in> (funs :: kzp set)"
+      by (simp add: NULL_kzp_def funs_kzp_def)
+
+    show "arity (NULL::kzp) = 0"
+      by (simp add: NULL_kzp_def)
+  qed
+end
+
+definition f :: "kzp wf_trm \<Rightarrow> kzp wf_trm" where
+  "f x \<equiv> Abs_wf_trm (App f_kzp [Rep_wf_trm x])"
+
+definition g :: "kzp wf_trm \<Rightarrow> kzp wf_trm \<Rightarrow> kzp wf_trm" where
+  "g x y \<equiv> Abs_wf_trm (App g_kzp [Rep_wf_trm x, Rep_wf_trm y])"
+
+definition P :: "kzp wf_trm \<Rightarrow> kzp skat" where
+  "P x \<equiv> pred (Abs_wf_pred (Pred P_kzp [x]))"
+
+definition vx :: "kzp wf_trm " where
+  "vx \<equiv> Abs_wf_trm (App x_kzp [])"
+
+definition bot :: "kzp wf_trm" where
+  "bot \<equiv> Abs_wf_trm (App bot_kzp [])"
+
+declare f_def [skat_simp]
+  and g_def [skat_simp]
+  and bot_def [skat_simp]
+  and P_def [skat_simp]
+  and vx_def [skat_simp]
+
+(* Sequences *)
+
+definition seq :: "'a::ranked_alphabet skat list \<Rightarrow> 'a skat" where
+  "seq xs = foldr op \<cdot> xs \<one>"
+
+declare seq_def [skat_simp]
+
+lemmas oner = skd.mult_oner[simplified]
+
+declare oner [skat_simp]
+
+lemma seq_singleton: "seq [v] = v"
+  by (simp add: seq_def, metis skd.mult_oner)
+
+lemma seq_mult: "seq (xs @ ys) = seq xs \<cdot> seq ys"
+  apply (induct xs)
+  apply (simp add: seq_def)
+  apply (metis skd.mult_onel)
+  apply (simp add: seq_def)
+  by (metis skd.mult_assoc)
+
+lemma list_td_split: "take n xs @ drop n xs = xs"
+  by (induct xs, simp_all)
+
+lemma seq_split:
+  assumes seq_take: "seq (take n xs) = seq (take n ys)"
+  and seq_drop: "seq (drop n xs) = seq (drop n ys)"
+  shows "seq xs = seq ys"
+proof -
+  have "seq (take n xs @ drop n xs) = seq (take n ys @ drop n ys)"
+    by (simp only: seq_mult, metis seq_drop seq_take)
+  thus ?thesis
+    by simp
+qed
+
+definition take_rev :: "nat \<Rightarrow> 'a list \<Rightarrow> 'a list" where
+  "take_rev n xs = rev (take n (rev xs))"
+
+declare take_rev_def [simp]
+
+definition drop_rev :: "nat \<Rightarrow> 'a list \<Rightarrow> 'a list" where
+  "drop_rev n xs = rev (drop n (rev xs))"
+
+declare drop_rev_def [simp]
+
+lemma take_drop_rev_id [simp]: "drop_rev n xs @ take_rev n xs = xs"
+  by (metis append_take_drop_id drop_rev_def rev_append rev_rev_ident take_rev_def)
+
+lemma seq_split_rev:
+  assumes seq_take: "seq (take_rev n xs) = seq (take_rev n ys)"
+  and seq_drop: "seq (drop_rev n xs) = seq (drop_rev n ys)"
+  shows "seq xs = seq ys"
+proof -
+  have "seq (drop_rev n xs @ take_rev n xs) = seq (drop_rev n ys @ take_rev n ys)"
+    by (simp only: seq_mult, metis seq_drop seq_take)
+  thus ?thesis
+    by (simp only: take_drop_rev_id)
+qed
+
+lemma seq_append:
+  "seq (take n xs) \<cdot> seq (drop n xs) = seq (take m ys) \<cdot> seq (drop m ys) \<Longrightarrow> seq xs = seq ys"
+  by (simp add: seq_mult[symmetric])
+
+abbreviation loop where "loop v \<equiv> skat_star (seq v)"
+
+(* Useful lemmas *)
+
+(* Sliding *)
+
+lemma seq_slide:
+  assumes xs_def: "xs = drop n ys"
+  shows "seq xs\<cdot>(seq ys)\<^sup>\<star> = (seq (xs @ take n ys))\<^sup>\<star>\<cdot>seq xs"
+proof -
+  have "seq xs \<cdot> (seq (take n ys) \<cdot> seq xs)\<^sup>\<star> = (seq xs \<cdot> seq (take n ys))\<^sup>\<star> \<cdot> seq xs"
+    by (simp add: ska.star_slide[simplified,symmetric])
+  thus ?thesis
+    by (metis append_take_drop_id assms seq_mult)
+qed
+
+(* Denesting *)
+
+definition APPEND :: "'a list \<Rightarrow> 'a list \<Rightarrow> 'a list" where
+  "APPEND \<alpha> \<beta> = \<alpha> @ \<beta>"
+
+lemma seq_denest_break: "x\<^sup>\<star>\<cdot>loop ys = x\<^sup>\<star>\<cdot>loop (APPEND (drop_rev n ys) (take_rev n ys))"
+  by (simp only: APPEND_def take_drop_rev_id)
+
+lemma seq_denest: "x\<^sup>\<star>\<cdot>loop (ys @ [x\<^sup>\<star>]) = (x + seq ys)\<^sup>\<star>"
+  by (metis seq_mult seq_singleton ska.star_denest_1 ska.star_denest_2 skat_order_def skd.add_comm)
+
+lemma seq_match: "\<lbrakk>x = y; seq xs = seq ys\<rbrakk> \<Longrightarrow> seq (x # xs) = seq (y # ys)"
+  by (metis (lifting) drop_1_Cons seq_split take_1_Cons)
+
+lemma seq_cut: "seq xs = seq (take n xs) \<cdot> seq (drop n xs)"
+  by (metis append_take_drop_id seq_mult)
+
+lemma seq_cut_app: "seq xs = seq (APPEND (take n xs) (drop n xs))"
+  by (simp add: APPEND_def)
+
+lemma seq_cut_app_rev: "seq xs = seq (APPEND (drop_rev n xs) (take_rev n xs))"
+  by (simp only: APPEND_def take_drop_rev_id)
+
+lemma seq_cut_rev: "seq xs = seq (drop_rev n xs) \<cdot> seq (take_rev n xs)"
+  by (metis seq_mult take_drop_rev_id)
+
+lemma seq_push: "y\<cdot>z = z\<cdot>y \<Longrightarrow> seq xs \<cdot> y \<cdot> seq (z#zs) = seq (xs @ [z]) \<cdot> y \<cdot> seq zs"
+proof -
+  assume yz_comm: "y \<cdot> z = z \<cdot> y"
+  have "seq xs \<cdot> y \<cdot> seq (z#zs) = seq xs \<cdot> (y \<cdot> z) \<cdot> seq zs"
+    by (metis append_Cons append_Nil seq_mult seq_singleton skd.mult_assoc)
+  also have "... = seq xs \<cdot> (z \<cdot> y) \<cdot> seq zs"
+    by (metis yz_comm)
+  also have "... = seq (xs @ [z]) \<cdot> y \<cdot> seq zs"
+    by (metis seq_mult seq_singleton skd.mult_assoc)
+  finally show ?thesis .
+qed
+
+lemma seq_head_comm: "x\<cdot>y = y\<cdot>x \<Longrightarrow> seq (x#y#xs) = seq (y#x#xs)"
+  by (metis (hide_lams, no_types) append_Cons append_Nil seq_mult seq_singleton)
+
+lemma seq_empty: "x = seq [] \<cdot> x"
+  by (simp add: seq_def skd.mult_onel)
+
+lemma seq_snoc: "seq xs \<cdot> x = seq (xs @ [x])"
+  by (metis seq_mult seq_singleton)
+
+lemma seq_cons: "x \<cdot> seq xs = seq (x#xs)"
+  by (metis append_Cons append_Nil seq_mult seq_singleton)
+
+lemma plus_indiv: "\<lbrakk>x1 = x2; y1 = y2\<rbrakk> \<Longrightarrow> (x1::kzp skat) + y1 = x2 + y2"
+  by auto
+
+lemma seq_plus_head_r: "seq xs = seq ys + seq zs \<Longrightarrow> seq (x#xs) = seq (x#ys) + seq (x#zs)"
+  by (metis append_Cons eq_Nil_appendI seq_mult skd.distl)
+
+lemma seq_plus_elim:
+  assumes pc: "p \<in> carrier tests"
+  shows "seq ((!p)#xs) + seq (p#xs) = seq xs"
+proof -
+  have "seq (!p#xs) + seq (p#xs) = !p \<cdot> seq xs + p \<cdot> seq xs"
+    by (simp add: seq_cons)
+  also have "... = (!p + p) \<cdot> seq xs"
+    by (metis skd.distr)
+  also have "... = \<one> \<cdot> seq xs"
+    sorry
+  also have "... = seq xs"
+    by (metis skd.mult_onel)
+  finally show ?thesis .
+qed
+
+lemma seq_permute: "\<lbrakk>xs \<in> set (permute ys); \<And>x y. \<lbrakk>x\<in>set xs; y \<in> set ys\<rbrakk> \<Longrightarrow> x\<cdot>y = y\<cdot>x\<rbrakk> \<Longrightarrow> seq xs = seq ys"
+  sorry
+
+lemma seq_zero: "last xs = !y \<Longrightarrow> seq xs \<cdot> seq(y#ys) = \<zero>"
+  sorry
+
+lemma seq_zero_var: "last xs \<cdot> y = \<zero> \<Longrightarrow> seq xs \<cdot> seq (y#ys) = \<zero>"
+  sorry
+
+lemma seq_shunt: "(\<forall>y\<in>set xs. x\<cdot>y = y\<cdot>x) \<Longrightarrow> seq (x#xs) = seq (xs@[x])"
+  sorry
+
+lemma seq_12: "seq (x#y#xs) = seq (x\<cdot>y#xs)"
+  sorry
+
+(* Shorthand notation *)
+
+definition a :: "nat \<Rightarrow> kzp skat" where
+  "a i \<equiv> P (var i)"
+
+abbreviation a1 where "a1 \<equiv> a 1"
+abbreviation a2 where "a2 \<equiv> a 2"
+abbreviation a3 where "a3 \<equiv> a 3"
+abbreviation a4 where "a4 \<equiv> a 4"
+
+declare a_def [skat_simp]
+
+lemma a_test: "a n \<in> carrier tests"
+  by (simp add: a_def P_def, rule pred_closed)
+
+lemma a_comm: "a n \<cdot> a m = a m \<cdot> a n" by skat_comm
+
+lemma a_assign: "n \<noteq> m \<Longrightarrow> a n \<cdot> m := x = m := x \<cdot> a n"
+  by (skat_comm, auto)
+
+definition b :: "nat \<Rightarrow> kzp skat" where
+  "b i \<equiv> P (f (var i))"
+
+declare b_def [skat_simp]
+
+definition c :: "nat \<Rightarrow> kzp skat" where
+  "c i \<equiv> P (f (f (var i)))"
+
+declare c_def [skat_simp]
+
+definition p :: "nat \<Rightarrow> nat \<Rightarrow> kzp skat" where
+  "p i j \<equiv> i := f (var j)"
+
+declare p_def [skat_simp]
+
+abbreviation p41 where "p41 \<equiv> p 4 1"
+abbreviation p11 where "p11 \<equiv> p 1 1"
+abbreviation p13 where "p13 \<equiv> p 1 3"
+abbreviation p22 where "p22 \<equiv> p 2 2"
+
+definition q :: "nat \<Rightarrow> nat \<Rightarrow> nat \<Rightarrow> kzp skat" where
+  "q i j k \<equiv> i := g (var j) (var k)"
+
+abbreviation q214 where "q214 \<equiv> q 2 1 4"
+abbreviation q311 where "q311 \<equiv> q 3 1 1"
+abbreviation q211 where "q211 \<equiv> q 2 1 1"
+
+declare q_def [skat_simp]
+
+definition r :: "nat \<Rightarrow> nat \<Rightarrow> kzp skat" where
+  "r i j \<equiv> i := f (f (var j))"
+
+abbreviation x1 where "x1 \<equiv> 1 := vx"
+
+definition s :: "nat \<Rightarrow> kzp skat" where
+  "s i \<equiv> i := f vx"
+
+definition t :: "nat \<Rightarrow> kzp skat" where
+  "t i \<equiv> i := g (f vx) (f vx)"
+
+definition u :: "nat \<Rightarrow> nat \<Rightarrow> nat \<Rightarrow> kzp skat" where
+  "u i j k \<equiv> i := g (f (f (var j))) (f (f (var k)))"
+
+definition z :: "nat \<Rightarrow> kzp skat" where
+  "z i \<equiv> 0 := var i"
+
+declare z_def [skat_simp]
+
+abbreviation z2 where "z2 \<equiv> z 2"
+
+definition y :: "nat \<Rightarrow> kzp skat" where
+  "y i \<equiv> i := bot"
+
+no_notation
+  one_class.one ("1") and
+  dioid.one ("1\<index>") and
+  dioid.zero ("0\<index>") and
+  zero_class.zero ("0") and
+  plus_class.plus (infixl "+" 65)
+
+definition scheme1 :: "kzp skat list" where "scheme1 \<equiv>
+  [ 1 := vx
+  , 4 := f (var 1)
+  , 1 := f (var 1)
+  , 2 := g (var 1) (var 4)
+  , 3 := g (var 1) (var 1)
+  , loop
+    [ !(P (var 1))
+    , 1 := f (var 1)
+    , 2 := g (var 1) (var 4)
+    , 3 := g (var 1) (var 1)
+    ]
+  , P (var 1)
+  , 1 := f (var 3)
+  , loop
+    [ !(P (var 4)) + seq
+      [ P (var 4)
+      , (!(P (var 2)) \<cdot> 2 := f (var 2))\<^sup>\<star>
+      , P (var 2)
+      , ! (P (var 3))
+      , 4 := f (var 1)
+      , 1 := f (var 1)
+      ]
+    , 2 := g (var 1) (var 4)
+    , 3 := g (var 1) (var 1)
+    , loop
+      [ !(P (var 1))
+      , 1 := f (var 1)
+      , 2 := g (var 1) (var 4)
+      , 3 := g (var 1) (var 1)
+      ]
+    , P (var 1)
+    , 1 := f (var 3)
+    ]
+  , P (var 4)
+  , (!(P (var 2)) \<cdot> 2 := f (var 2))\<^sup>\<star>
+  , P (var 2)
+  , P (var 3)
+  , 0 := var 2
+  , halt
+  ]"
+
+definition scheme2 where "scheme2 \<equiv>
+  [ 2 := f vx
+  , P (var 2)
+  , 2 := g (var 2) (var 2)
+  , skat_star (seq
+    [ !(P (var 2))
+    , 2 := f (f (var 2))
+    , P (var 2)
+    , 2 := g (var 2) (var 2)
+    ])
+  , P (var 2)
+  , 0 := var 2
+  , halt
+  ]"
+
+declare Nat.One_nat_def [simp del]
+declare foldr.simps[skat_simp]
+declare o_def[skat_simp]
+declare id_def[skat_simp]
+
+lemma kozen1: "p41\<cdot>p11 = p41\<cdot>p11\<cdot>(a1 iff a4)"
+  sorry
+
+lemma kozen2: "p41\<cdot>p11\<cdot>q214 = p41\<cdot>p11\<cdot>q211"
+  sorry
+
+theorem kozen_scheme_equivalence: "seq scheme1 = seq scheme2"
+proof -
+  have "seq scheme1 = seq
+    [x1,p41,p11,q214,q311,loop [!a1,p11,q214,q311]
+    ,loop [a1,p13,!a4 + seq [a4,(!a2\<cdot>p22)\<^sup>\<star>,a2,!a3,p41,p11],q214,q311,loop [!a1,p11,q214,q311]]
+    ,a1,p13,a4,(!a2\<cdot>p22)\<^sup>\<star>,a2,a3,z2,halt]"
+    apply (simp add: scheme1_def p_def[symmetric] q_def[symmetric] a_def[symmetric] z_def[symmetric])
+    apply (rule seq_split[of 6], simp_all)
+    apply (rule seq_split[of 3], simp_all)
+    apply (rule seq_append[of 2 _ 1], simp)
+    apply (simp only: seq_singleton)
+    apply (rule HOL.trans)
+    by (rule seq_slide[of _ 4], simp_all)
+
+  also have "... = seq
+    [x1,p41,p11,q214,q311
+    ,(seq [!a1,p11,q214,q311] + seq [a1,p13,!a4 + seq [a4,(!a2\<cdot>p22)\<^sup>\<star>,a2,!a3,p41,p11],q214,q311])\<^sup>\<star>
+    ,a1,p13,a4,(!a2\<cdot>p22)\<^sup>\<star>,a2,a3,z2,halt]"
+    apply (rule seq_split[of 5])
+    apply simp_all
+    apply (rule seq_split_rev[of 8])
+    apply simp_all
+    apply (subst seq_def, simp)
+    apply (subst skd.mult_oner[simplified])
+    apply (subst seq_denest_break[of _ _ 1])
+    apply simp
+    apply (simp only: APPEND_def)
+    apply (subst seq_denest)
+    by (simp only: seq_singleton)
+
+  also have "... = seq
+    [x1,p41,p11,q214,q311
+    ,(seq [!a1,p11,q214,q311] + seq [a1,p13,!a4,q214,q311] + seq [a1,p13,a4,(!a2\<cdot>p22)\<^sup>\<star>,a2,!a3,p41,p11,q214,q311])\<^sup>\<star>
+    ,a1,p13,a4,(!a2\<cdot>p22)\<^sup>\<star>,a2,a3,z2,halt]"
+    apply (rule seq_split[of 5], simp_all)
+    apply (rule seq_split_rev[of 8], simp_all)
+    apply (simp add: seq_singleton)
+    apply (subst skd.add_assoc[simplified])
+    apply (rule_tac f = "\<lambda>x. (?v + x)\<^sup>\<star>" in arg_cong)
+    apply (simp add: seq_def skd.mult_oner)
+    apply (subst skd.distr[simplified])
+    apply (simp add: skd.mult_assoc[symmetric, simplified])
+    apply (subst skd.distl[simplified])
+    by (simp add: skd.mult_assoc[simplified])
+
+  also have "... = seq
+    [x1,p41,p11,q214,q311
+    ,(seq [!a1,!a4,p11,q214,q311] + seq [!a1,a4,p11,q214,q311] + seq [a1,!a4,p13,q214,q311]
+    + seq [a1,a4,p13,(!a2\<cdot>p22)\<^sup>\<star>,a2,!a3,p41,p11,q214,q311])\<^sup>\<star>
+    ,(!a2\<cdot>p22)\<^sup>\<star>,a1,a2,a3,a4,z2,halt]"
+    apply (rule seq_split[of 5], simp_all)
+    apply (rule seq_match)
+    apply (rule arg_cong) back
+    apply (rule plus_indiv)+
+    apply (rule seq_plus_head_r)
+    apply (subst seq_plus_elim)
+    apply (rule a_test, simp)
+    apply (rule seq_split[of 1], simp_all)
+    apply (rule seq_split_rev[of 2], simp_all)
+    apply (simp add: seq_def skd.mult_oner)
+    apply skat_comm
+    apply (rule seq_split[of 1], simp_all)
+    apply (rule seq_split_rev[of 7], simp_all)
+    apply (simp add: seq_def)
+    apply skat_comm
+    apply (subst seq_head_comm) back
+    apply skat_comm
+    apply (subst seq_split[of 1], simp_all)
+    apply (subgoal_tac "halt = p13 \<cdot> halt")
+    apply (erule ssubst) back
+    apply (subst seq_cut[of _ 1], simp_all)
+    apply (subst seq_def, simp add: skd.mult_oner[simplified])
+    apply (subst seq_empty)
+    apply (subst seq_push, skat_comm)+
+    apply (subst skd.mult_assoc[simplified])
+    apply (subst seq_snoc)
+    apply (simp add: seq_singleton)
+    apply (subst seq_split_rev[of 2], simp_all)
+    apply (subst seq_head_comm, skat_comm, subst seq_split[of 1], simp_all)+
+    apply (subst skat_halt[of 1]) back
+    apply (simp add: output_vars_kzp_def)
+    apply (simp add: p_def)
+    apply (subst skd.mult_assoc[symmetric,simplified])
+    apply (subst skat_null_zero)
+    apply (subst skat_halt[symmetric])
+    apply (simp add: output_vars_kzp_def)
+    by simp
+
+  also have "... = seq
+    [x1,p41,p11,q214,q311
+    ,(seq [!a1,a4,p11,q214,q311]
+    + seq [a1,a4,p13,(!a2\<cdot>p22)\<^sup>\<star>,a2,!a3,p41,p11,q214,q311])\<^sup>\<star>
+    ,(!a2\<cdot>p22)\<^sup>\<star>,a1,a2,a3,a4,z2,halt]"
+    apply (subst seq_split[of 5], simp_all)
+    apply (subst seq_cons[symmetric])
+    apply (subst seq_cons[symmetric]) back back back back back
+    apply (subst skd.add_assoc[simplified])
+    apply (subst skd.add_comm[simplified]) back
+    apply (subst skd.add_assoc[symmetric,simplified])
+    apply (subst skd.add_assoc[simplified]) back
+    apply (rule ska.kozen_skat_lemma[simplified])
+    apply (subgoal_tac "seq [!a1,!a4,p11,q214,q311] = seq [!a1,p11,q214,q311,!a4]")
+    apply (erule ssubst)
+    apply (subgoal_tac "seq [a1,!a4,p13,q214,q311] = seq [a1,p13,q214,q311,!a4]")
+    apply (erule ssubst)
+    apply (subst seq_head_comm) back back
+    apply skat_comm
+    apply (subst seq_head_comm) back back back
+    apply skat_comm
+    apply (simp add: skd.distr[simplified] skd.distl[simplified])
+    apply (subst seq_zero, simp)+
+    apply (simp add: skd.add_zerol)
+    prefer 3
+    apply (subgoal_tac "seq [(!a2\<cdot>p22)\<^sup>\<star>,a1,a2,a3,a4,z2,halt] = seq [a4,(!a2\<cdot>p22)\<^sup>\<star>,a1,a2,a3,z2,halt]")
+    apply (erule ssubst)
+    apply (subgoal_tac "seq [!a1,!a4,p11,q214,q311] = seq [!a1,p11,q214,q311,!a4]")
+    apply (erule ssubst)
+    apply (subgoal_tac "seq [a1,!a4,p13,q214,q311] = seq [a1,p13,q214,q311,!a4]")
+    apply (erule ssubst)
+    apply (simp add: skd.distr[simplified])
+    apply (subst seq_zero,simp)+
+    apply (simp add: skd.add_zerol)
+    prefer 3
+    apply (subst seq_head_comm) back
+    apply skat_comm
+    apply (subst seq_split[of 1], simp_all)
+    apply (subst seq_split_rev[of 2], simp_all)
+    apply (rule seq_permute)
+    apply simp
+    apply (simp, safe)
+    apply skat_comm+
+    apply (subst seq_split[of 1], simp_all)
+    apply (subst seq_shunt, simp, safe, skat_comm+, simp)
+    apply (subst seq_split[of 1], simp_all)
+    by (subst seq_shunt, simp, safe, skat_comm+, simp)
+
+  also have "... = seq
+    [x1,p41,p11,q214,q311
+    ,(seq [a1,a4,p13,(!a2\<cdot>p22)\<^sup>\<star>,a2,!a3,p41,p11,q214,q311])\<^sup>\<star>
+    ,(!a2\<cdot>p22)\<^sup>\<star>,a1,a2,a3,a4,z2,halt]"
+    apply (subst seq_split_rev[of 7], simp_all)
+    apply (subst seq_def)
+    apply (subst seq_def) back back
+    apply (simp add: skd.mult_assoc[symmetric,simplified] skd.mult_oner[simplified])
+    apply (rule ska.kozen_skat_lemma_dual[simplified])
+    defer
+    apply (subst skd.mult_assoc[simplified])
+    apply (subst kozen1)
+    apply (simp add: skd.mult_assoc[symmetric,simplified])
+    apply (subst seq_empty)
+    apply (subst seq_snoc)+
+    apply (subst seq_snoc[symmetric])
+    apply simp
+    apply (subst seq_cut[of _ 3], simp)
+    apply (subst seq_shunt) back
+    apply (simp, safe)
+    apply skat_comm+
+    apply simp
+    apply (subst seq_12) back back
+    apply (subst skd.mult_assoc[simplified])
+    apply (subst seq_zero_var)
+    apply (simp add: biconditional_def)
+    defer
+    apply (metis skd.mult_zeror)
+    apply (subst seq_cut[of _ 6], simp)
+    apply (subst seq_cut[of _ 2]) back apply simp
+    apply (subst seq_def) back
+    apply (simp add: skd.mult_oner[simplified])
+    apply (subst kozen1)
+    apply (subst skd.mult_assoc[simplified]) back
+    apply (subst seq_cons)
+    apply (simp add: skd.mult_assoc[simplified])
+    apply (subst seq_shunt) back
+    apply (simp, safe)
+    apply skat_comm+
+    apply simp
+    apply (subst seq_12) back back
+    apply (subst seq_zero_var)
+    apply simp
+    prefer 2
+    apply (simp add: skd.mult_zeror[simplified])
+    apply (simp add: biconditional_def)
+    sorry
+
+  also have "... = seq
+    [x1,p41,p11,q211,q311
+    ,(seq [a1,a4,p13,(!a2\<cdot>p22)\<^sup>\<star>,a2,!a3,p41,p11,q211,q311])\<^sup>\<star>
+    ,(!a2\<cdot>p22)\<^sup>\<star>,a1,a2,a3,a4,z2,halt]"
+    apply (simp add: seq_def)
+    apply (simp add: skd.mult_assoc[symmetric,simplified] skd.mult_oner[simplified])
+    by (smt kozen2 skd.mult_assoc)
+    
+
+  also have "... = seq scheme2"
+    sorry
+
+  finally show ?thesis .
+qed
+
+end
